
 \section{Chi-Square Distribution}


\subsection{Non-Central Chi-Square}



\subsection{Moment Generating Function}

We can get MGF for chi-square from $E[x^2 t]$ and $E[(\mu + Z)^2 t]$, where $Z \sim N(0,1)$.
Let's prove it in two methods:
\begin{itemize}
	\item [(i)] Method 1:
	
	\begin{align*}
		M_i(t) &= E[x^2 t] = \frac{1}{\sqrt{2\pi}} \int exp(x^2 t) exp \left( - \frac{(x-\mu)^2}{2} \right) dx\\
		&=  \frac{1}{\sqrt{2\pi}}  \int exp \left( (t- \frac{1}{2}) x^2 + \mu x -\frac{\mu^2}{2} \right) dx \\
		&=  \frac{1}{\sqrt{2\pi}}  \int exp \left(  -\frac{1}{2}(1-2t) \{ x^2 - \frac{2 \mu x}{(1-2t)} + \frac{\mu^2}{(1-2t)^2} \} + \frac{\mu^2}{2(1-2t)} -\frac{\mu^2}{2}  \right) dx \\
		&= \frac{1}{\sqrt{(1-2t)}} \int \frac{(1-2t)}{\sqrt{2\pi}} exp\left( -\frac{(x-\frac{\mu}{1-2t})^2}{2 (1-2t)^{-1}} \right) dx \left[exp \left( \frac{\mu^2 t}{1-2t} \right) \right]\\
		&=\frac{1}{\sqrt{(1-2t)}} exp \left( \frac{\mu^2 t}{1-2t} \right), \qquad \lambda = \mu^2\\
		&=\frac{1}{\sqrt{(1-2t)}} exp \left( \frac{\lambda t}{1-2t} \right)
	\end{align*}
	
	Then the MGF for $Q_i \sim \chi^2 _{k_i}(\lambda_i)$
	\begin{align*}
		M(t) &= E[ \sum_{i=1}^k x_i^2 t] = \prod_{i=1}^k M_i(t) \\
		&=\left(\frac{1}{\sqrt{(1-2t)}} \right)^k exp \left( \frac{ \sum_{i=1}^k \lambda_i t }{1-2t} \right)\\
		&=\left(\frac{1}{\sqrt{(1-2t)}} \right)^k exp \left( \frac{ \lambda t }{1-2t} \right)\\
		&= (1-2t)^{-k/2} exp \left( \frac{ \lambda t }{1-2t} \right), \qquad \text{i.i.d}
	\end{align*}
	
	\item[(ii)] Method 2:
	
	\begin{align*}
	M(t) &= E[(\mu + Z)^2 t] = \frac{1}{\sqrt{2\pi}} \int exp \left((\mu + Z)^2 t \right) exp \left( - \frac{Z^2}{2} \right) dz\\
	&=  \frac{1}{\sqrt{2\pi}}  \int exp \left( (t- \frac{1}{2}) z^2 + 2\mu t z + \mu^2 t \right) dz \\
	&=  \frac{1}{\sqrt{2\pi}}  \int exp \left(  -\frac{(1-2t)}{2} \{ z^2 - \frac{4 \mu t z}{(1-2t)} + \frac{2 \mu^2 t^2}{(1-2t)^2} \} + \frac{2 \mu^2 t^2}{(1-2t)} + \mu^2 t   \right) dz \\
	&= \frac{1}{\sqrt{(1-2t)}} \left[exp \left( \frac{\mu^2 t}{1-2t} \right) \right] \int \frac{1}{\sqrt{2\pi/(1-2t)}} exp\left( -\frac{(z-\frac{2 \mu t}{1-2t})^2}{2 (1-2t)^{-1}} \right) dz \\
	&=\frac{1}{\sqrt{(1-2t)}} exp \left( \frac{\mu^2 t}{1-2t} \right), \qquad t<1/2
\end{align*}


\end{itemize}

The general case of a linear combination of independent $\chi^2_{k_i}(\lambda_i)$

\begin{align*}
	Q &= \sum_{i=1}^k a_i Q_i
\end{align*}
We also can prove using MGF.

\subsection{Linear Combination of Chi-Square Distribution}

The linear combination of chi-square distribution $Y_j$. Let us denote by $X \sim \Gamma(r, \lambda)$ the fact that the r.v. X has a Gamma distribution with shape parameter r and rate parameter $\lambda$ 

\begin{align*}
	f_{X}(x) &= \frac{\lambda^x}{\Gamma (r)} exp(- \lambda x) x^{r-1}, \qquad (r, \lambda >0, x >0)
\end{align*}

Then we have, for $j=1,..p$,

\begin{align*}
	Y_j & \sim  \Gamma(\frac{k_j}{2}, \frac{1}{2}) \rightarrow Z_j = w_j Y_j \sim \Gamma(\frac{k_j}{2}, \frac{1}{2w_j})
\end{align*}

The MGF for linear combinations $Z_j = w_j Y_j$
\begin{align*}
	M(t) &= E[exp(Y_j t)] = (1-2t)^{-k/2} exp \left( \frac{ \lambda t }{1-2t} \right)\\
	M_{Z_j} (t) & = E[exp(w_j Y_j t)] = E[exp( Y_j (w_jt))] \\
	&= (1-2 w_jt)^{-1/2} exp \left( \frac{ \lambda w_j t }{1-2 w_j t} \right)
\end{align*}

\begin{align*}
	M_Y(t) &= E[exp(Y t)] = E[exp(t [w_1 Y_1 + w_2 Y_2 + w_3 Y_3 +.. w_n Y_n])]\\
	&= E[exp(w_1 t Y_1)]E[exp(w_2 t Y_2)]... E[exp(w_n t Y_n)]\\
	&= M_{X_1}(w_1 t) M_{X_2}(w_2 t) M_{X_3}(w_3 t).. M_{X_n}(w_n t)\\
	&= \prod_{i=1}^n M_{X_i}(w_i t)
\end{align*}

The third equation comes from the properties of exponents, as wells as from the expectation of the product of functions of independent random variables. 

I need to pay attention that, only under independent and identical situation, we can write
 \begin{align*}
 	M_Y(t) &= M_{X}(t)^n
 \end{align*}

Other than that, we can not further simplify that. So back to the non-central chi-square distribution, we have the MGF of Y
\begin{align*}
	M_Y(t) &= \prod_{i=1}^n M_{X_i}(w_i t)\\
	&=\prod_{i=1}^n  (1-2 w_jt)^{-1/2} exp \left( \frac{ \lambda w_j t }{1-2 w_j t} \right)
\end{align*}

Then we can see that the shape parameter is $\frac{1}{2 w_i}$. If we want to have a non-central chi-square distribution for $Y$, then all $w_j$ need to be the same. 

 